@prefix : <http://w3id.org/bodi#> .
@prefix dc: <http://purl.org/dc/elements/1.1/> .
@prefix ns: <http://creativecommons.org/ns#> .
@prefix owl: <http://www.w3.org/2002/07/owl#> .
@prefix rdf: <http://www.w3.org/1999/02/22-rdf-syntax-ns#> .
@prefix xml: <http://www.w3.org/XML/1998/namespace> .
@prefix xsd: <http://www.w3.org/2001/XMLSchema#> .
@prefix bodi: <http://w3id.org/bodi#> .
@prefix prov: <http://www.w3.org/ns/prov#> .
@prefix rdfs: <http://www.w3.org/2000/01/rdf-schema#> .
@prefix rico: <https://www.ica.org/standards/RiC/ontology#> .
@prefix skos: <http://www.w3.org/2004/02/skos/core#> .
@prefix vann: <http://purl.org/vocab/vann/> .
@prefix terms: <http://purl.org/dc/terms/> .
@prefix premis: <http://www.loc.gov/premis/rdf/v3/> .
@base <http://w3id.org/bodi#> .

<http://w3id.org/bodi#> rdf:type owl:Ontology ;
                         owl:imports <http://iflastandards.info/ns/lrm/lrmoo/> ,
                                     <https://id.loc.gov/ontologies/premis-3-0-0> ,
                                     <https://www.ica.org/standards/RiC/ontology/1.1> ;
                         dc:contributor "Francesca Tomasi" ,
                                        "Paolo Bonora" ;
                         dc:creator "Lucia Giagnolini" ;
                         dc:title "BoDi (Born-Digital) Ontology" ;
                         terms:created "2025-10-01" ;
                         terms:description "An extension of RiC-O (Records in Contexts Ontology) designed to represent the complexity of born-digital archival materials, addressing requirements for technical metadata, digital provenance, integrity verification, and contextual relationships." ;
                         terms:license "This work is distributed under a Creative Commons Attribution License (https://creativecommons.org/licenses/by/4.0/)." ;
                         vann:preferredNamespacePrefix "bodi" ;
                         vann:preferredNamespaceUri "http://w3id.org/bodi#" ;
                         owl:versionIRI "http://w3id.org/bodi/1.0" ;
                         owl:versionInfo 1.0 .

#################################################################
#    Annotation properties
#################################################################

###  http://purl.org/dc/terms/created
terms:created rdf:type owl:AnnotationProperty .


###  http://purl.org/dc/terms/license
terms:license rdf:type owl:AnnotationProperty .


###  http://w3id.org/bodi#sameContentCount
bodi:sameContentCount rdf:type owl:AnnotationProperty ;
                      rdfs:comment "Count of Records with identical content - files sharing the same hash code indicate byte-for-byte identical content." ;
                      rdfs:label "Same content count" .


###  http://www.w3.org/2002/07/owl#versionIRI
owl:versionIRI rdf:type owl:AnnotationProperty .


#################################################################
#    Object Properties
#################################################################

###  http://w3id.org/bodi#generatedBy
bodi:generatedBy rdf:type owl:ObjectProperty ;
                 rdfs:subPropertyOf rico:isRelatedTo ;
                 owl:inverseOf bodi:hasGenerated ;
                 rdfs:domain owl:Thing ;
                 rdfs:range [ rdf:type owl:Class ;
                              owl:unionOf ( rico:Activity
                                            rico:Agent
                                          )
                            ] ;
                 rdfs:comment "Indicates that a resource was created, produced, or brought into existence by a specific Agent or Activity. This property establishes a creation relationship between any resource and the agent pr activity responsible for its generation, whether through automated processes, human intervention, or hybrid approaches." ;
                 rdfs:label "Generated by" .


###  http://w3id.org/bodi#hasFileClusterPosition
bodi:hasFileClusterPosition rdf:type owl:ObjectProperty ;
                            rdfs:subPropertyOf rico:isRelatedTo ;
                            owl:inverseOf bodi:isFileClusterPositionOf ;
                            rdfs:domain rico:Instantiation ;
                            rdfs:range bodi:FileClusterPosition ;
                            rdfs:comment "Links a logical instantiation of a digital resource to its corresponding physical allocation on the storage medium." ;
                            rdfs:label "Has file cluster position" .


###  http://w3id.org/bodi#hasGenerated
bodi:hasGenerated rdf:type owl:ObjectProperty ;
                  rdfs:subPropertyOf rico:isRelatedTo ;
                  rdfs:domain [ rdf:type owl:Class ;
                                owl:unionOf ( rico:Activity
                                              rico:Agent
                                            )
                              ] ;
                  rdfs:range owl:Thing ;
                  rdfs:comment "Indicates that an Agent or Activity has created, produced, or brought into existence a specific resource. This property represents the inverse relationship of 'generatedBy', allowing navigation from agents and activities to their generated outputs." ;
                  rdfs:label "Has generated" .


###  http://w3id.org/bodi#hasHashCode
bodi:hasHashCode rdf:type owl:ObjectProperty ;
                 rdfs:subPropertyOf rico:isRelatedTo ;
                 owl:inverseOf bodi:isHashCodeOf ;
                 rdfs:domain rico:Instantiation ;
                 rdfs:range premis:Fixity ;
                 rdfs:comment "Associates an instantiation with its cryptographic hash code or checksum value. This property is crucial for digital preservation workflows, enabling integrity verification, duplicate detection, and authenticity validation of digital resources over time." ;
                 rdfs:label "Has hash code" .


###  http://w3id.org/bodi#hasOrHadSupervisor
bodi:hasOrHadSupervisor rdf:type owl:ObjectProperty ;
                        rdfs:subPropertyOf rico:isOrWasUnderAuthorityOf ;
                        owl:inverseOf bodi:isOrWasSupervisorOf ;
                        rdfs:domain rico:Activity ;
                        rdfs:range rico:Agent ;
                        rdfs:comment "Indicates that an activity is or was supervised, managed, or overseen by a specific Agent. This property captures both current and historical supervisory relationships, essential for tracking accountability and governance in digital preservation workflows." ;
                        rdfs:label "Has or had supervisor" .


###  http://w3id.org/bodi#hasRevisioned
bodi:hasRevisioned rdf:type owl:ObjectProperty ;
                   rdfs:subPropertyOf rico:isRelatedTo ;
                   owl:inverseOf bodi:revisedBy ;
                   rdfs:domain rico:Agent ;
                   rdfs:range bodi:TechnicalDescription ;
                   rdfs:comment "Connects a Person to the AI Generated Text that she has revised." ;
                   rdfs:label "Has revisioned" .


###  http://w3id.org/bodi#hasSameHashCodeAs
bodi:hasSameHashCodeAs rdf:type owl:ObjectProperty ;
                       rdfs:subPropertyOf rico:isInstantiationAssociatedWithInstantiation ;
                       rdf:type owl:SymmetricProperty ;
                       rdfs:domain rico:Instantiation ;
                       rdfs:range rico:Instantiation ;
                       rdfs:comment "Establishes that two digital instantiations have identical hash codes, indicating they are likely exact digital copies or duplicates." ;
                       rdfs:label "Has same hash code as" .


###  http://w3id.org/bodi#hasSoftwareComponent
bodi:hasSoftwareComponent rdf:type owl:ObjectProperty ;
                          rdfs:subPropertyOf rico:hasOrHadPart ;
                          owl:inverseOf bodi:isSoftwareComponentOf ;
                          rdfs:domain bodi:Software ;
                          rdfs:range bodi:SoftwareComponent ;
                          rdfs:comment "Indicates that a Software contains or includes a specific Software Component as one of its constituent parts. This property helps model the hierarchical structure of complex software environments." ;
                          rdfs:label "Has Software Component" .


###  http://w3id.org/bodi#hasStackElement
bodi:hasStackElement rdf:type owl:ObjectProperty ;
                     rdfs:subPropertyOf rico:hasOrHadPart ;
                     owl:inverseOf bodi:isStackElementOf ;
                     rdfs:domain bodi:SoftwareStack ;
                     rdfs:range rico:Mechanism ;
                     rdfs:comment "Indicates that a software stack includes a specific Mechanism as one of its constituent elements. This property allows for modeling the various components (Software, Algorithms, Software Components) that together form a complete technological stack responsible for some Activity." ;
                     rdfs:label "Has stack element" .


###  http://w3id.org/bodi#hasStorageLocation
bodi:hasStorageLocation rdf:type owl:ObjectProperty ;
                        rdfs:subPropertyOf rico:isRelatedTo ;
                        owl:inverseOf bodi:isStorageLocationOf ;
                        rdfs:domain owl:Thing ;
                        rdfs:range premis:StorageLocation ;
                        rdfs:comment "Connects an Entity to the Storage Location in which is located." ;
                        rdfs:label "Has Storage Location" .


###  http://w3id.org/bodi#hasTechnicalDescription
bodi:hasTechnicalDescription rdf:type owl:ObjectProperty ;
                             rdfs:subPropertyOf rico:isRelatedTo ;
                             owl:inverseOf bodi:isTechnicalDescriptionOf ;
                             rdfs:domain owl:Thing ;
                             rdfs:range bodi:TechnicalDescription ;
                             rdfs:comment "Links an instantiation to its technical description, which provides detailed information about the technical characteristics, structure, format, or implementation details of the resource." ;
                             rdfs:label "Has technical description" .


###  http://w3id.org/bodi#hasTechnicalDescriptionType
bodi:hasTechnicalDescriptionType rdf:type owl:ObjectProperty ;
                                 rdfs:subPropertyOf rico:hasOrHadType ;
                                 owl:inverseOf bodi:isTechnicalDescriptionTypeOf ;
                                 rdfs:domain bodi:TechnicalDescription ;
                                 rdfs:range bodi:TechnicalDescriptionType ;
                                 rdfs:comment "Connects a Technical Description to a Technical Description Type that defines it." ;
                                 rdfs:label "Has Technical Description Type" .


###  http://w3id.org/bodi#hasTechnicalMetadata
bodi:hasTechnicalMetadata rdf:type owl:ObjectProperty ;
                          rdfs:subPropertyOf rico:isRelatedTo ;
                          owl:inverseOf bodi:isTechnicalMetadataOf ;
                          rdfs:domain rico:Instantiation ;
                          rdfs:range bodi:TechnicalMetadata ;
                          rdfs:comment "Associates an Instantiation with technical metadata that describes its technical properties, format specifications, creation parameters, or other characteristics." ;
                          rdfs:label "Has Technical Metadata" .


###  http://w3id.org/bodi#hasTechnicalMetadataType
bodi:hasTechnicalMetadataType rdf:type owl:ObjectProperty ;
                              rdfs:subPropertyOf rico:hasOrHadType ;
                              owl:inverseOf bodi:isTechnicalMetadataTypeOf ;
                              rdfs:domain bodi:TechnicalMetadata ;
                              rdfs:range bodi:TechnicalMetadataType ;
                              rdfs:comment "Connects a Technical Metadata to its Type" ;
                              rdfs:label "Has technical metadata type" .


###  http://w3id.org/bodi#isFileClusterPositionOf
bodi:isFileClusterPositionOf rdf:type owl:ObjectProperty ;
                             rdfs:subPropertyOf rico:isRelatedTo ;
                             rdfs:domain bodi:FileClusterPosition ;
                             rdfs:range rico:Instantiation ;
                             rdfs:comment "Associates a physical file cluster position with the logical instantiation  whose data it stores on the medium." .


###  http://w3id.org/bodi#isHashCodeOf
bodi:isHashCodeOf rdf:type owl:ObjectProperty ;
                  rdfs:subPropertyOf rico:isRelatedTo ;
                  rdfs:domain premis:Fixity ;
                  rdfs:range rico:Instantiation ;
                  rdfs:comment "Associates a cryptographic hash code or checksum value with the instantiation it identifies. This property supports digital preservation workflows by linking the integrity marker back to the corresponding digital resource, ensuring traceability, verification, and authenticity validation." ;
                  rdfs:label "Is Hash Code Of" .


###  http://w3id.org/bodi#isOrWasSupervisorOf
bodi:isOrWasSupervisorOf rdf:type owl:ObjectProperty ;
                         rdfs:subPropertyOf rico:hasOrHadAuthorityOver ;
                         rdfs:domain rico:Agent ;
                         rdfs:range rico:Activity ;
                         rdfs:comment "Indicates that an Agent supervises, manages, or oversees a specific Activity. This property reflects the Agent’s role in providing oversight and guidance, and it is essential for documenting responsibility, authority, and governance within digital preservation workflows." ;
                         rdfs:label "Is or was supervisor of" .


###  http://w3id.org/bodi#isSoftwareComponentOf
bodi:isSoftwareComponentOf rdf:type owl:ObjectProperty ;
                           rdfs:subPropertyOf rico:isOrWasPartOf ;
                           rdfs:domain bodi:SoftwareComponent ;
                           rdfs:range bodi:Software ;
                           rdfs:comment "Indicates that a Software Component is part of a Software Stack as one of its constituent elements. This property supports the representation of hierarchical structures within complex software environments, linking individual components to the encompassing Software." ;
                           rdfs:label "Is software component of" .


###  http://w3id.org/bodi#isStackElementOf
bodi:isStackElementOf rdf:type owl:ObjectProperty ;
                      rdfs:subPropertyOf rico:isOrWasPartOf ;
                      rdfs:domain rico:Mechanism ;
                      rdfs:range bodi:SoftwareStack ;
                      rdfs:comment "Indicates that a Mechanism is part of a software stack as one of its constituent elements. This property links individual components (Software, Algorithms, Software Components) to the broader technological stack of which they form a part, supporting the modeling of composite systems responsible for carrying out an Activity." ;
                      rdfs:label "Is stack element of" .


###  http://w3id.org/bodi#isStorageLocationOf
bodi:isStorageLocationOf rdf:type owl:ObjectProperty ;
                         rdfs:subPropertyOf rico:isRelatedTo ;
                         rdfs:domain premis:StorageLocation ;
                         rdfs:range owl:Thing ;
                         rdfs:comment "Connects a Storage Location to the Entity in which is located." ;
                         rdfs:label "is Storage Location Of" .


###  http://w3id.org/bodi#isTechnicalDescriptionOf
bodi:isTechnicalDescriptionOf rdf:type owl:ObjectProperty ;
                              rdfs:subPropertyOf rico:isRelatedTo ;
                              rdfs:domain bodi:TechnicalDescription ;
                              rdfs:range owl:Thing ;
                              rdfs:comment "Links a technical description to the Instantiation is referred to." ;
                              rdfs:label "Is Technical Description Of" .


###  http://w3id.org/bodi#isTechnicalDescriptionTypeOf
bodi:isTechnicalDescriptionTypeOf rdf:type owl:ObjectProperty ;
                                  rdfs:subPropertyOf rico:isOrWasTypeOf ;
                                  rdfs:domain bodi:TechnicalDescriptionType ;
                                  rdfs:range bodi:TechnicalDescription ;
                                  rdfs:comment "Connects a Technical Descption Type to a Technical Description it defines." ;
                                  rdfs:label "Is Technical Description Type Of" .


###  http://w3id.org/bodi#isTechnicalMetadataOf
bodi:isTechnicalMetadataOf rdf:type owl:ObjectProperty ;
                           rdfs:subPropertyOf rico:isRelatedTo ;
                           rdfs:domain bodi:TechnicalMetadata ;
                           rdfs:range rico:Instantiation ;
                           rdfs:comment "Associates a Technical Metadata to the Instatiation is referred to." ;
                           rdfs:label "is Technical Metadata Of" .


###  http://w3id.org/bodi#isTechnicalMetadataTypeOf
bodi:isTechnicalMetadataTypeOf rdf:type owl:ObjectProperty ;
                               rdfs:subPropertyOf rico:isOrWasTypeOf ;
                               rdfs:domain bodi:TechnicalMetadataType ;
                               rdfs:range bodi:TechnicalMetadata ;
                               rdfs:comment "Connects a Technical Metadata Type to its related Technical Metadata" ;
                               rdfs:label "Is Technical Metadata Type Of" .


###  http://w3id.org/bodi#revisedBy
bodi:revisedBy rdf:type owl:ObjectProperty ;
               rdfs:subPropertyOf rico:isRelatedTo ;
               rdfs:domain bodi:TechnicalDescription ;
               rdfs:range rico:Agent ;
               rdfs:comment "Connects an AI Generated Text to the Person that revisioned the information." ;
               rdfs:label "Revised by" .


###  https://www.ica.org/standards/RiC/ontology#hasOrHadPart
rico:hasOrHadPart rdf:type owl:ObjectProperty ;
                  rdfs:subPropertyOf rico:isRelatedTo .


###  https://www.ica.org/standards/RiC/ontology#hasOrHadType
rico:hasOrHadType rdf:type owl:ObjectProperty ;
                  rdfs:subPropertyOf rico:isRelatedTo .


###  https://www.ica.org/standards/RiC/ontology#isInstantiationAssociatedWithInstantiation
rico:isInstantiationAssociatedWithInstantiation rdf:type owl:ObjectProperty ;
                                                rdfs:subPropertyOf rico:isRelatedTo .


###  https://www.ica.org/standards/RiC/ontology#isOrWasPartOf
rico:isOrWasPartOf rdf:type owl:ObjectProperty ;
                   rdfs:subPropertyOf rico:isRelatedTo .


###  https://www.ica.org/standards/RiC/ontology#isOrWasTypeOf
rico:isOrWasTypeOf rdf:type owl:ObjectProperty ;
                   rdfs:subPropertyOf rico:isRelatedTo .


###  https://www.ica.org/standards/RiC/ontology#isRelatedTo
rico:isRelatedTo rdf:type owl:ObjectProperty .


#################################################################
#    Data properties
#################################################################

###  http://w3id.org/bodi#confidenceScore
bodi:confidenceScore rdf:type owl:DatatypeProperty ;
                     rdfs:domain bodi:TechnicalDescription ;
                     rdfs:range xsd:decimal ;
                     rdfs:comment "A numerical value between 0 and 10 indicating the confidence level or reliability of AI-generated text. Higher values indicate greater confidence in the accuracy or quality of the generated content, supporting quality assessment and validation workflows." ;
                     rdfs:label "Confindence score" .


###  http://w3id.org/bodi#exceptionMessage
bodi:exceptionMessage rdf:type owl:DatatypeProperty ;
                      rdfs:domain bodi:Exception ;
                      rdfs:range rdfs:Literal ;
                      rdfs:comment "Contains the error message or description associated with an exception that occurred during processing. This property is essential for logging, debugging, and understanding failures in automated workflows." ;
                      rdfs:label "Exception message" .


###  http://w3id.org/bodi#hasDocumentation
bodi:hasDocumentation rdf:type owl:DatatypeProperty ;
                      rdfs:domain rico:Thing ;
                      rdfs:range xsd:anyURI ;
                      rdfs:comment "Provides a URI reference to official documentation, specifications, manuals, or other authoritative sources that describe the resource." ;
                      rdfs:label "Has documentation" .


###  http://w3id.org/bodi#hasHumanValidation
bodi:hasHumanValidation rdf:type owl:DatatypeProperty ;
                        rdfs:domain bodi:TechnicalDescription ;
                        rdfs:range rdfs:Literal ;
                        rdfs:comment "Indicates whether AI-generated text has been reviewed, verified, or validated by human experts. This property is crucial for quality assurance in systems that combine automated processing with human oversight." ;
                        rdfs:label "Has human validation" .


###  http://w3id.org/bodi#hierarchyDepth
bodi:hierarchyDepth rdf:type owl:DatatypeProperty ;
                    rdfs:domain rico:Instantiation ;
                    rdfs:range xsd:integer ;
                    rdfs:comment "Specifies the numerical depth level of a resource within a directory or organizational hierarchy, with level 0 representing the root." ;
                    rdfs:label "Hierarchy depth" .


###  http://w3id.org/bodi#redactedInformation
bodi:redactedInformation rdf:type owl:DatatypeProperty ;
                         rdfs:subPropertyOf owl:topDataProperty ;
                         rdfs:domain rico:RecordResource ;
                         rdfs:range rdfs:Literal ;
                         rdfs:comment "Indication of whether or not the resource has been anonymized." ;
                         rdfs:label "Redacted information" .


#################################################################
#    Classes
#################################################################

###  http://w3id.org/bodi#Algorithm
bodi:Algorithm rdf:type owl:Class ;
               rdfs:subClassOf rico:Mechanism ;
               rdfs:comment "A computational procedure, formula, or set of rules designed to perform a specific task or solve a particular problem." ;
               rdfs:label "Algorithm" .


###  http://w3id.org/bodi#Exception
bodi:Exception rdf:type owl:Class ;
               rdfs:subClassOf rico:Concept ;
               rdfs:comment "An error condition, unexpected event, or abnormal situation that occurs during the execution of digital preservation processes. Exceptions are important for system monitoring, quality control, and troubleshooting automated workflows." ;
               rdfs:label "Exception" .


###  http://w3id.org/bodi#FileClusterPosition
bodi:FileClusterPosition rdf:type owl:Class ;
                         rdfs:subClassOf rico:Thing ;
                         rdfs:comment "Represents the physical allocation of a digital file’s data on a storage medium. It captures the material trace of a digital document at the level of bit distribution across clusters or sectors of the device." ;
                         rdfs:label "File cluster position" .


###  http://w3id.org/bodi#Software
bodi:Software rdf:type owl:Class ;
              rdfs:subClassOf premis:SoftwareAgent ,
                              rico:Mechanism ;
              rdfs:comment "A computer program, application, or digital tool that performs specific functions. Software entities are characterized by their functionality, version information, and technical specifications." ;
              rdfs:label "Software" .


###  http://w3id.org/bodi#SoftwareComponent
bodi:SoftwareComponent rdf:type owl:Class ;
                       rdfs:subClassOf rico:Mechanism ;
                       rdfs:comment "A modular, reusable part of a software system that provides specific functionality and can be combined with other components to create larger applications." ;
                       rdfs:label "Software component" .


###  http://w3id.org/bodi#SoftwareStack
bodi:SoftwareStack rdf:type owl:Class ;
                   rdfs:subClassOf rico:Agent ;
                   owl:disjointWith rico:Mechanism ;
                   rdfs:comment "A collection of mechanisms that performs an Activity together to provide a solution for a specific task." ;
                   rdfs:label "Software Stack" .


###  http://w3id.org/bodi#TechnicalDescription
bodi:TechnicalDescription rdf:type owl:Class ;
                          rdfs:subClassOf rico:Concept ;
                          rdfs:comment "Technical Description of the Instantiation generated by humans, by artificial intelligence (AI), or through a hybrid approach (AI-generated and human-revised)." ;
                          rdfs:label "AI generated text" .


###  http://w3id.org/bodi#TechnicalDescriptionType
bodi:TechnicalDescriptionType rdf:type owl:Class ;
                              rdfs:subClassOf rico:Type ;
                              rdfs:comment "The type of Technical Description, e.g. a description note on the file format." ;
                              rdfs:label "Technical Description Type" .


###  http://w3id.org/bodi#TechnicalMetadata
bodi:TechnicalMetadata rdf:type owl:Class ;
                       rdfs:subClassOf rico:Concept ;
                       rdfs:comment "The actual value or content of technical metadata associated with a digital resource. For example, in 'cp:revision = 1', the value '1' represents the TechnicalMetadata instance, while 'cp:revision' is the Technical Metadata Type. These values describe specific technical characteristics such as format parameters, creation settings, and other measurable attributes." ;
                       rdfs:label "Technical metadata" .


###  http://w3id.org/bodi#TechnicalMetadataType
bodi:TechnicalMetadataType rdf:type owl:Class ;
                           rdfs:subClassOf rico:Type ;
                           rdfs:comment "The type, property, or category that defines what kind of technical metadata is being described. For example, in 'cp:revision = 1', 'cp:revision' represents the TechnicalMetadataType that categorizes the metadata as revision information. This classification enables systematic organization of different kind of metadata like version identifiers, format specifications, encoding parameters, and preservation characteristics." ;
                           rdfs:label "Technical Metadata Type" .


###  http://w3id.org/bodi#TechnicalMetadataTypeSet
bodi:TechnicalMetadataTypeSet rdf:type owl:Class ;
                              rdfs:subClassOf rico:Concept ;
                              rdfs:comment "Group of Technical Metadata Types" ;
                              rdfs:label "Technical Metadata Type Set" .


###  http://www.loc.gov/premis/rdf/v3/Fixity
premis:Fixity rdf:type owl:Class .


###  http://www.loc.gov/premis/rdf/v3/SoftwareAgent
premis:SoftwareAgent rdf:type owl:Class .


###  http://www.loc.gov/premis/rdf/v3/StorageLocation
premis:StorageLocation rdf:type owl:Class .


###  http://www.w3.org/ns/prov#Entity
prov:Entity rdf:type owl:Class .


###  https://www.ica.org/standards/RiC/ontology#Activity
rico:Activity rdf:type owl:Class ;
              rdfs:subClassOf rico:Thing .


###  https://www.ica.org/standards/RiC/ontology#Agent
rico:Agent rdf:type owl:Class ;
           rdfs:subClassOf rico:Thing .


###  https://www.ica.org/standards/RiC/ontology#Concept
rico:Concept rdf:type owl:Class ;
             rdfs:subClassOf rico:Thing .


###  https://www.ica.org/standards/RiC/ontology#Extent
rico:Extent rdf:type owl:Class ;
            rdfs:subClassOf rico:Thing .


###  https://www.ica.org/standards/RiC/ontology#Instantiation
rico:Instantiation rdf:type owl:Class ;
                   rdfs:subClassOf prov:Entity ,
                                   rico:Thing .


###  https://www.ica.org/standards/RiC/ontology#Mechanism
rico:Mechanism rdf:type owl:Class ;
               rdfs:subClassOf rico:Agent .


###  https://www.ica.org/standards/RiC/ontology#RecordResource
rico:RecordResource rdf:type owl:Class ;
                    rdfs:subClassOf prov:Entity ,
                                    rico:Thing .


###  https://www.ica.org/standards/RiC/ontology#Thing
rico:Thing rdf:type owl:Class .


###  https://www.ica.org/standards/RiC/ontology#Type
rico:Type rdf:type owl:Class ;
          rdfs:subClassOf rico:Thing .


###  Generated by the OWL API (version 4.5.26.2023-07-17T20:34:13Z) https://github.com/owlcs/owlapi
